examples/machine-code/instruction-set-models/x86_64/x64_icacheScript.sml
@@ -10,28 +10,28 @@ val _ = new_theory "x64_icache";
 (* instruction cache definitions *)
 
 val X64_ICACHE_def = Define `
-  X64_ICACHE ((r,e,s,t,m,i):x64_state) ((r2,e2,s2,t2,m2,i2):x64_state) =
+  X64_ICACHE ((r,e,s,m,i):x64_state) ((r2,e2,s2,m2,i2):x64_state) =
     ?insert delete.
-      (r = r2) /\ (e = e2) /\ (s = s2) /\ (t = t2) /\ (m = m2) /\
+      (r = r2) /\ (e = e2) /\ (s = s2) /\ (m = m2) /\
       (i2 = \addr. if addr IN insert then m addr else
                    if addr IN delete then NONE else i addr)`;
 
 val X64_ACCURATE_def = Define `
-  X64_ACCURATE a ((r,e,s,t,m,i):x64_state) = (i a = NONE) \/ (i a = m a)`;
+  X64_ACCURATE a ((r,e,s,m,i):x64_state) = (i a = NONE) \/ (i a = m a)`;
 
 val icache_def = Define `
   icache (insert,delete) m i addr =
     if addr IN insert then m addr else if addr IN delete then NONE else i addr`;
 
 val X64_ICACHE_UPDATE_def = Define `
-  X64_ICACHE_UPDATE x ((r1,e1,s1,t1,m1,i1):x64_state) = (r1,e1,s1,t1,m1,icache x m1 i1)`;
+  X64_ICACHE_UPDATE x ((r1,e1,s1,m1,i1):x64_state) = (r1,e1,s1,m1,icache x m1 i1)`;
 
 
 (* theorems *)
 
 val X64_ICACHE_REFL = store_thm("X64_ICACHE_REFL",
   ``!s. X64_ICACHE s s``,
-  STRIP_TAC THEN `?r e t t' m i. s = (r,e,t,t',m,i)` by METIS_TAC [PAIR]
+  STRIP_TAC THEN `?r e t m i. s = (r,e,t,m,i)` by METIS_TAC [PAIR]
   THEN ASM_SIMP_TAC std_ss [X64_ICACHE_def]
   THEN Q.EXISTS_TAC `{}` THEN Q.EXISTS_TAC `{}`
   THEN ASM_SIMP_TAC std_ss [NOT_IN_EMPTY,FUN_EQ_THM]);
@@ -39,9 +39,9 @@ val X64_ICACHE_REFL = store_thm("X64_ICACHE_REFL",
 val X64_ICACHE_TRANS = store_thm("X64_ICACHE_TRANS",
   ``!s t u. X64_ICACHE s t /\ X64_ICACHE t u ==> X64_ICACHE s u``,
   REPEAT STRIP_TAC
-  THEN `?r1 e1 t1 t1' m1 i1. s = (r1,e1,t1,t1',m1,i1)` by METIS_TAC [PAIR]
-  THEN `?r2 e2 t2 t2' m2 i2. t = (r2,e2,t2,t2',m2,i2)` by METIS_TAC [PAIR]
-  THEN `?r3 e3 t3 t3' m3 i3. u = (r3,e3,t3,t3',m3,i3)` by METIS_TAC [PAIR]
+  THEN `?r1 e1 t1 m1 i1. s = (r1,e1,t1,m1,i1)` by METIS_TAC [PAIR]
+  THEN `?r2 e2 t2 m2 i2. t = (r2,e2,t2,m2,i2)` by METIS_TAC [PAIR]
+  THEN `?r3 e3 t3 m3 i3. u = (r3,e3,t3,m3,i3)` by METIS_TAC [PAIR]
   THEN FULL_SIMP_TAC std_ss [X64_ICACHE_def,FUN_EQ_THM]
   THEN REPEAT (POP_ASSUM (K ALL_TAC))
   THEN Q.EXISTS_TAC `insert' UNION (insert DIFF delete')`
@@ -49,9 +49,9 @@ val X64_ICACHE_TRANS = store_thm("X64_ICACHE_TRANS",
   THEN SIMP_TAC std_ss [IN_DIFF,IN_INSERT,IN_UNION] THEN METIS_TAC []);
 
 val X64_ICACHE_THM = store_thm("X64_ICACHE_THM",
-  ``X64_ICACHE (r,e,s,t,m,i) (r2,e2,s2,t2,m2,i2) =
+  ``X64_ICACHE (r,e,s,m,i) (r2,e2,s2,m2,i2) =
     ?update.
-      (r2,e2,s2,t2,m2,i2) = (r,e,s,t,m,icache update m i)``,
+      (r2,e2,s2,m2,i2) = (r,e,s,m,icache update m i)``,
   SIMP_TAC std_ss [EXISTS_PROD,X64_ICACHE_def,icache_def,FUN_EQ_THM]
   THEN METIS_TAC []);
 
@@ -62,38 +62,27 @@ val ZREAD_CLAUSES = store_thm("ZREAD_CLAUSES",
         (ZREAD_REG r (ZCLEAR_ICACHE s) = ZREAD_REG r s) /\
         (ZREAD_REG r (X64_ICACHE_UPDATE u s) = ZREAD_REG r s) /\
         (ZREAD_REG r (ZWRITE_MEM2 a x s) = ZREAD_REG r s) /\
-        (ZREAD_REG r (ZWRITE_STACK t s) = ZREAD_REG r s) /\
         (ZREAD_RIP (ZWRITE_REG r2 w s) = ZREAD_RIP s) /\
         (ZREAD_RIP (ZWRITE_RIP e s) = e) /\
         (ZREAD_RIP (ZWRITE_EFLAG f b s) = ZREAD_RIP s) /\
         (ZREAD_RIP (ZCLEAR_ICACHE s) = ZREAD_RIP s) /\
         (ZREAD_RIP (X64_ICACHE_UPDATE u s) = ZREAD_RIP s) /\
         (ZREAD_RIP (ZWRITE_MEM2 a x s) = ZREAD_RIP s) /\
-        (ZREAD_RIP (ZWRITE_STACK t s) = ZREAD_RIP s) /\
-        (ZREAD_STACK (ZWRITE_REG r2 w s) = ZREAD_STACK s) /\
-        (ZREAD_STACK (ZWRITE_RIP e s) = ZREAD_STACK s) /\
-        (ZREAD_STACK (ZWRITE_EFLAG f b s) = ZREAD_STACK s) /\
-        (ZREAD_STACK (ZCLEAR_ICACHE s) = ZREAD_STACK s) /\
-        (ZREAD_STACK (X64_ICACHE_UPDATE u s) = ZREAD_STACK s) /\
-        (ZREAD_STACK (ZWRITE_MEM2 a x s) = ZREAD_STACK s) /\
-        (ZREAD_STACK (ZWRITE_STACK t s) = t) /\
         (ZREAD_EFLAG i (ZWRITE_REG r2 w s) = ZREAD_EFLAG i s) /\
         (ZREAD_EFLAG i (ZWRITE_RIP e s) = ZREAD_EFLAG i s) /\
         (ZREAD_EFLAG i (ZWRITE_EFLAG f b s) = if f = i then b else ZREAD_EFLAG i s) /\
         (ZREAD_EFLAG i (ZCLEAR_ICACHE s) = ZREAD_EFLAG i s) /\
         (ZREAD_EFLAG i (X64_ICACHE_UPDATE u s) = ZREAD_EFLAG i s) /\
         (ZREAD_EFLAG i (ZWRITE_MEM2 a x s) = ZREAD_EFLAG i s) /\
-        (ZREAD_EFLAG i (ZWRITE_STACK t s) = ZREAD_EFLAG i s) /\
         (ZREAD_MEM2 a (ZWRITE_REG r2 w s) = ZREAD_MEM2 a s) /\
         (ZREAD_MEM2 a (ZWRITE_RIP e s) = ZREAD_MEM2 a s) /\
         (ZREAD_MEM2 a (ZWRITE_EFLAG f b s) = ZREAD_MEM2 a s) /\
         (ZREAD_MEM2 a (ZCLEAR_ICACHE s) = ZREAD_MEM2 a s) /\
         (ZREAD_MEM2 a (X64_ICACHE_UPDATE u s) = ZREAD_MEM2 a s) /\
-        (ZREAD_MEM2 a (ZWRITE_MEM2 c x s) = if a = c then x else ZREAD_MEM2 a s) /\
-        (ZREAD_MEM2 a (ZWRITE_STACK t s) = ZREAD_MEM2 a s)``,
-  STRIP_TAC THEN `?r2 e2 s2 t2 m2 i2. s = (r2,e2,s2,t2,m2,i2)` by METIS_TAC [pairTheory.PAIR]
+        (ZREAD_MEM2 a (ZWRITE_MEM2 c x s) = if a = c then x else ZREAD_MEM2 a s)``,
+  STRIP_TAC THEN `?r2 e2 s2 m2 i2. s = (r2,e2,s2,m2,i2)` by METIS_TAC [pairTheory.PAIR]
   THEN Cases_on `u`
-  THEN ASM_SIMP_TAC std_ss [ZREAD_REG_def,ZREAD_RIP_def,ZREAD_STACK_def,ZWRITE_STACK_def,
+  THEN ASM_SIMP_TAC std_ss [ZREAD_REG_def,ZREAD_RIP_def,
          ZREAD_EFLAG_def, ZWRITE_REG_def, ZWRITE_MEM2_def, ZREAD_MEM2_def,
          combinTheory.APPLY_UPDATE_THM, ZWRITE_RIP_def,CAN_ZREAD_MEM,
          ZWRITE_EFLAG_def,ZCLEAR_ICACHE_def,CAN_ZWRITE_MEM,X64_ICACHE_UPDATE_def]
